Start passing precondition to circ append

src/program_proof/wal/logger_proof.v
@@ -91,6 +91,11 @@ Proof.
   iFrameNamed. auto.
 Qed.
 
+(** log_inv is the resources exclusively owned by the logger thread *)
+Definition log_inv γ σₛ: iProp Σ :=
+  "HnotLogging" ∷ thread_own γ.(diskEnd_avail_name) Available ∗
+  "Happender" ∷ is_circular_appender γ.(circ_name) σₛ.(circ).
+
 Theorem wp_Walog__logAppend l γ σₛ :
   {{{ "#HmemLock" ∷ readonly (l ↦[Walog.S :: "memLock"] #σₛ.(memLock)) ∗
       "#HcondLogger" ∷ readonly (l ↦[Walog.S :: "condLogger"] #σₛ.(condLogger)) ∗
@@ -101,9 +106,11 @@ Theorem wp_Walog__logAppend l γ σₛ :
       "#His_cond2" ∷ is_cond σₛ.(condInstall) #σₛ.(memLock) ∗
       "#?" ∷ readonly (l ↦[Walog.S :: "st"] #σₛ.(wal_st)) ∗
       "#His_lock" ∷ is_lock N γ.(lock_name) #σₛ.(memLock) (wal_linv σₛ.(wal_st) γ) ∗
+      "#Hwal" ∷ inv N (∃ σ, is_wal_inner l γ σ ∗ P σ) ∗
+      "#Hcirc" ∷ is_circular circN (circular_pred γ) γ.(circ_name) ∗
       "Hlkinv" ∷ wal_linv σₛ.(wal_st) γ ∗
       "Hlocked" ∷ locked γ.(lock_name) ∗
-      "HnotLogging" ∷ thread_own γ.(diskEnd_avail_name) Available
+      "Hlogger" ∷ log_inv γ σₛ
   }}}
     Walog__logAppend #l
   {{{ (progress:bool), RET #progress;
@@ -113,6 +120,7 @@ Theorem wp_Walog__logAppend l γ σₛ :
   }}}.
 Proof.
   iIntros (Φ) "Hpre HΦ"; iNamed "Hpre".
+  iNamed "Hlogger".
   wp_call.
   wp_apply (wp_Walog__waitForSpace with "[$Hlkinv $Hlocked]").
   { iFrameNamed. iFrame "#". }
@@ -134,17 +142,23 @@ Proof.
   }
   iNamed "HdiskEnd_circ".
   iMod (thread_own_get with "HdiskEnd_exactly HnotLogging") as "(HdiskEnd_exactly&HdiskEnd_is&HareLogging)".
+  iNamed "Hstart_circ".
   wp_loadField.
-  wp_apply (release_spec with "[-HΦ HareLogging $His_lock $Hlocked]").
+  wp_apply (release_spec with "[-HΦ HareLogging HdiskEnd_is Happender Hbufs $His_lock $Hlocked]").
   { iExists _; iFrame "# ∗".
     iExists _; iFrame "% ∗". }
   wp_loadField. wp_loadField.
-  (* wp_apply wp_circular__Append. *)
+  wp_apply (wp_circular__Append with "[$Hbufs $HdiskEnd_is $Happender $Hcirc $Hstart_at_least]").
+  { admit. }
+  { admit. }
 Admitted.
 
 Theorem wp_Walog__logger l γ :
   {{{ "#Hwal" ∷ is_wal P l γ ∗
-      "HnotLogging" ∷ thread_own γ.(diskEnd_avail_name) Available }}}
+      thread_own γ.(diskEnd_avail_name) Available
+      (* TODO: for is_circular_appender, probably should just not put c in Walog
+      but as local variable in logger *)
+  }}}
     Walog__logger #l
   {{{ RET #(); True }}}.
 Proof.
@@ -169,7 +183,11 @@ Proof.
     wp_if_destruct.
     - wp_pures.
       wp_apply (wp_Walog__logAppend with "[$Hlkinv $Hlk_held $HnotLogging]").
-      { iFrame "#". }
+      { iFrame "# ∗".
+        iDestruct "Hwal" as "[Hwal Hcirc]".
+        iFrame "#".
+        admit.
+      }
       iIntros (progress) "(Hlkinv&Hlk_held&HnotLogging)".
       wp_pures.
       destruct (negb progress); [ wp_if_true | wp_if_false ]; wp_pures.
@@ -189,6 +207,6 @@ Proof.
   wp_loadField.
   wp_apply (release_spec with "[$lk $Hlk_held $Hlkinv]").
   iApply ("HΦ" with "[//]").
-Qed.
+Admitted.
 
 End goose_lang.
